A perfect stack implementation. Along comes array too, which gives some insights into the way stack push operations have to be specified.

src/programs/stack.dfy
@@ -37,55 +37,59 @@ function stack_depth(s: Stack) : int
     s.stk.Length
 }
 
-method stack_push(s: Stack, d: int) returns (rstack: Stack, res: Result)
+function stack_peek(s: Stack) : Result
     requires s.stk != null;
-    requires s.stk.Length > 0;
-    requires s.top >= -1;
-    ensures (s.stk.Length > (s.top + 1)) ==> (rstack.top == s.top + 1) &&
-                                              (rstack.stk == s.stk) && 
-                                              rstack.stk.Length > rstack.top == (s.top+1) >= 0 &&
-                                              (rstack.stk[rstack.top] == d) && 
-                                              (res == Result(d, OK));
-    
-    ensures (s.stk.Length == (s.top + 1)) ==> /*(s == old(s)) && (rstack == old(s)) && 
-                                              s.top == old(s.top) && s.stk == old(s.stk) &&
-                                              rstack.stk[rstack.top] == s.stk[s.top] &&*/
-                                              rstack == old(s) && s == old(s) && 
-                                              res == Result(0, FULL);
-    modifies s.stk;
+    requires s.stk.Length > s.top >= -1;
+    reads s.stk;
 {
-    if (s.stk.Length > (s.top + 1)) {
-        s.stk[s.top + 1] := d;
-        rstack := Stack(s.stk, s.top + 1);
-        res := Result(d, OK);
-    } else {
-        rstack := s;
-        res := Result(0, FULL);
-    }
+    if (s.top > -1) then
+        Result(s.stk[s.top], OK)
+     else
+        Result(0, EMPTY)
 }
 
-method stack_pop(s: Stack) returns (rstack: Stack, res: Result)
+function stack_full(s: Stack) : bool
+    requires s.stk != null;
+    requires s.stk.Length > s.top >= -1;
+    reads s.stk;
+{
+    (s.top + 1 == s.stk.Length)
+}
+
+function stack_empty(s: Stack) : bool
+    requires s.stk != null;
+    requires s.stk.Length > s.top >= -1;
+    reads s.stk;
+{
+    (s.top == -1)
+}
+
+method stack_push_safe(s: Stack, d: int) returns (rstack: Stack, res: Result)
+    requires s.stk != null;
+    requires s.stk.Length > 0;
+    requires s.stk.Length > (s.top + 1) >= 0;
+    
+    modifies s.stk;
+    ensures rstack == Stack(s.stk, s.top+1);
+    ensures forall k :: 0 <= k < rstack.top ==> (rstack.stk[k] == old(s.stk[k]));
+    ensures rstack.stk[rstack.top] == d;
+    ensures res == Result(d, OK);
+{
+    s.stk[s.top + 1] := d;
+    rstack := Stack(s.stk, s.top+1);
+    res := Result(d, OK);
+}
+
+function method stack_pop_safe(s: Stack) : Stack
     requires s.stk != null;
     requires s.top >= -1;
     requires s.stk.Length > 0;
     requires s.stk.Length > s.top;
-    ensures (s.stk.Length > s.top > -1) ==> 
-                             (rstack == Stack(s.stk, s.top - 1)) &&
-                             (res == Result(s.stk[s.top], OK));
-
-    ensures (s.top == -1) ==> (rstack == s) &&
-                              (res == Result(0, EMPTY));
 {
-    if (s.top > -1) {
-        res := Result(s.stk[s.top], OK);
-        rstack := Stack(s.stk, s.top - 1);
-    } else {
-         rstack := s;
-         res := Result(0, EMPTY);
-    }
+    if (s.top > -1) then Stack(s.stk, s.top - 1) else s
 }
 
-method test_one_element_stack()
+method test_one_element_stack_safe()
 {
     var stk := stack_new(1);
     var rstk, res;
@@ -93,27 +97,29 @@ method test_one_element_stack()
     assert(stk.stk != null);
     assert(stack_size(stk) == 0);
 
-    rstk, res := stack_push(stk, 10);
+    rstk, res := stack_push_safe(stk, 10);
     assert(stack_size(rstk) == 1);
     assert(status(res) == OK);
     assert(val(res) == 10);
     assert(stack_size(rstk) == stack_size(stk) + 1);
     assert(rstk.stk[rstk.top] == 10);
+    assert(stack_peek(rstk).status == OK);
+    assert(stack_peek(rstk).data == 10);
 
-    rstk, res := stack_push(rstk, 20);
-    assert(stack_size(rstk) == 1);
-    assert(val(res) == 0 && status(res) == FULL);
-    assert(rstk.stk != null && rstk.stk == stk.stk);
-    assert(rstk.stk[rstk.top] == 10);
+    assert(stack_full(rstk));
 
-    rstk, res := stack_pop(rstk);
+    rstk := stack_pop_safe(rstk);
     assert(stack_size(rstk) == 0);
-    assert(status(res) == OK);
-//    assert(val(res) == 10);
 
+    assert(stack_empty(rstk));
+    rstk, res := stack_push_safe(rstk, 20);
+    assert(stack_peek(rstk).data == 20);
+    
+    rstk := stack_pop_safe(rstk);
+    assert(stack_empty(rstk));
 }
 
-method test_one_element_stack_push_pop()
+method test_one_element_stack_push_pop_safe()
 {
     var stk := stack_new(1);
     var rstk, res;
@@ -121,37 +127,43 @@ method test_one_element_stack_push_pop()
     assert(stk.stk != null);
     assert(stack_size(stk) == 0);
 
-    rstk, res := stack_push(stk, 10);
+    rstk, res := stack_push_safe(stk, 10);
     assert(stack_size(rstk) == 1);
     assert(status(res) == OK);
     assert(val(res) == 10);
     assert(stack_size(rstk) == stack_size(stk) + 1);
     assert(rstk.stk[rstk.top] == 10);
 
-    rstk, res := stack_pop(rstk);
+    rstk := stack_pop_safe(rstk);
     assert(stack_size(rstk) == 0);
-    assert(status(res) == OK);
-    assert(val(res) == 10);
+    assert(stack_empty(rstk));
 
-    rstk, res := stack_pop(rstk);
+    rstk := stack_pop_safe(rstk);
     assert(stack_size(rstk) == 0);
-    assert(status(res) == EMPTY);
-    assert(val(res) == 0);
+    assert(stack_empty(rstk));
 
-    rstk, res := stack_push(stk, 20);
+    rstk := stack_pop_safe(rstk);
+    assert(stack_size(rstk) == 0);
+    assert(stack_empty(rstk));
+
+    rstk, res := stack_push_safe(stk, 20);
     assert(stack_size(rstk) == 1);
     assert(status(res) == OK);
     assert(val(res) == 20);
     assert(stack_size(rstk) == stack_size(stk) + 1);
     assert(rstk.stk[rstk.top] == 20);
 
-    rstk, res := stack_pop(rstk);
+    rstk, res := stack_push_safe(stk, 20);
+    rstk, res := stack_push_safe(stk, 20);
+    rstk, res := stack_push_safe(stk, 20);
+
+    rstk := stack_pop_safe(rstk);
     assert(stack_size(rstk) == 0);
-    assert(status(res) == OK);
-    assert(val(res) == 20);
+    assert(stack_empty(rstk));
 }
 
-method test_two_element_stack()
+
+method test_two_element_stack_safe()
 {
     var stk := stack_new(2);
     var rstk, res;
@@ -159,20 +171,68 @@ method test_two_element_stack()
     assert(stk.stk != null);
     assert(stack_size(stk) == 0);
 
-    rstk, res := stack_push(stk, 10);
+    rstk, res := stack_push_safe(stk, 10);
+    rstk, res := stack_push_safe(rstk, 20);
+    assert(stack_peek(rstk).data == 20);
+    assert(stack_size(rstk) == 2);
+    assert(stack_depth(rstk) == 2);
+    assert(stack_full(rstk));
+
+    rstk:= stack_pop_safe(rstk);
+    assert(!stack_empty(rstk));
+    assert(stack_size(rstk) == 1);
+    assert(stack_peek(rstk).data == 10);
+    rstk := stack_pop_safe(rstk);
+    assert(stack_empty(rstk));
+    rstk := stack_pop_safe(rstk);
+    assert(stack_empty(rstk));
+}
+
+method test_generic_stack()
+{
+    var stk := stack_new(4);
+    var rstk, res;
+
+    assert(stk.stk != null);
+    assert(stack_size(stk) == 0);
+
+    rstk, res := stack_push_safe(stk, 10);
     assert(stack_size(rstk) == 1);
     assert(status(res) == OK);
     assert(val(res) == 10);
     assert(stack_size(rstk) == stack_size(stk) + 1);
 
-    rstk, res := stack_push(rstk, 20);
-    assert(stack_size(rstk) == 2);
-    assert(status(res) == OK);
-    assert(val(res) == 20);
-    assert(stack_size(rstk) == stack_size(stk) + 2);
+    assert(stack_peek(rstk).data == 10);
+    rstk := stack_pop_safe(rstk);
+    assert(stack_size(rstk) == 0);
 
-    rstk, res := stack_push(rstk, 30);
-    assert(val(res) == 0 && status(res) == FULL);
-    assert(stack_size(rstk) == 2);
+    rstk, res := stack_push_safe(rstk, 30);
+    rstk, res := stack_push_safe(rstk, 20);
+
+    assert(stack_peek(rstk).data == 20);
+    rstk := stack_pop_safe(rstk);
+    assert(stack_size(rstk) == 1);
+    assert(stack_peek(rstk).data == 30);
+    rstk := stack_pop_safe(rstk);
+    assert(stack_size(rstk) == 0);
+
+    rstk := stack_pop_safe(rstk);
+    assert(stack_size(rstk) == 0);
+
+    rstk, res := stack_push_safe(rstk, 25); assert(res.status == OK);
+    rstk, res := stack_push_safe(rstk, 50); assert(res.status == OK);
+    rstk, res := stack_push_safe(rstk, 75); assert(res.status == OK);
+    rstk, res := stack_push_safe(rstk, 100); assert(res.status == OK);
+    assert(stack_full(rstk));
+    //rstk, res := stack_push_safe(rstk, 100); // precondition doesn't hold!
+
+    assert(stack_peek(rstk).data == 100);
+    rstk := stack_pop_safe(rstk);
+    rstk := stack_pop_safe(rstk);
+    assert(stack_peek(rstk).data == 50);
+    rstk := stack_pop_safe(rstk);
+    assert(stack_peek(rstk).data == 25);
+    rstk := stack_pop_safe(rstk);
+    assert(stack_empty(rstk));
 }
 
